@prefix : <http://ns.jasnell.me/social#> .
@prefix s: <http://ns.jasnell.me/social#> .
@prefix owl: <http://www.w3.org/2002/07/owl#> .
@prefix rdf: <http://www.w3.org/1999/02/22-rdf-syntax-ns#> .
@prefix xml: <http://www.w3.org/XML/1998/namespace> .
@prefix xsd: <http://www.w3.org/2001/XMLSchema#> .
@prefix rdfs: <http://www.w3.org/2000/01/rdf-schema#> .
@base <http://www.w3.org/ns/activitystreams> .

<http://ns.jasnell.me/social#> a owl:Ontology ;
  rdfs:comment "Social Artifacts"@en ;
  rdfs:label "Social Artifacts"@en .

:Population a owl:Class ;
  rdfs:label "Population"@en ;
  rdfs:subClassOf owl:Class .

:Everyone a :Population ;
  rdfs:label "Everyone"@en ;
  rdfs:comment "Represents the subset of a total population that is visible to the context."@en .

:Public a :Population ;
  rdfs:label "Public"@en ;
  rdfs:comment "Represents the subset of a total population that is both visible to the context and shares a publicly known or visible relationship with the context"@en .

:Private a :Population ;
  rdfs:label "Private"@en ;
  rdfs:comment "Represents the subset of a total population that is both visible to the context and shares a private or publicly invisible relationship with the context"@en .

:Direct a :Population ;
  rdfs:label "Direct"@en ;
  rdfs:comment "Represents the subset of a total population that is both visible to the context and directly connected to the context"@en .

:Common a :Population ;
  rdfs:label "Common"@en ;
  rdfs:comment "Represents the subset of a total population that is both visible to the context and is determined to share common attributes with the context"@en .

:Interested a :Population ;
  rdfs:label "Interested"@en ;
  rdfs:comment "Represnts the subset of a total population that is both visible to the context and has an express interest in the context"@en .

:Self a :Population ;
  rdfs:label "Self"@en ;
  rdfs:comment "Represents the context resource itself as a member of the total population"@en .

:All a :CompoundPopulation ;
  rdfs:label "All"@en;
  rdfs:comment "Represents the subset represented by the intersection of multiple subsets (that is, members must belong to all specified subsets"@en .

:Any a :CompoundPopulation ;
  rdfs:label "Any"@en;
  rdfs:comment "Represents the subset represented by the union of multiple subsets (that is, members must belong to any of the specified subsets"@en .

:None a :CompoundPopulation ;
  rdfs:label "None"@en;
  rdfs:comment "Represents the subset represented by the complement of multiple subsets (that is, members must not belong to any of the specified subsets"@en .

:CompoundPopulation a owl:Class ;
  rdfs:label "CompoundPopulation"@en ;
  rdfs:comment "A population composed of multiple sub-populations."@en ;
  rdfs:subClassOf rdf:Bag, :Population .

:member a owl:ObjectProperty, rdfs:ContainerMembershipProperty ;
  rdfs:label "member"@en;
  rdfs:subPropertyOf rdfs:member ;
  rdfs:domain :CompoundPopulation ;
  rdfs:range :Population ;

:havingDimension a owl:ObjectProperty ;
  rdfs:label "havingDimension"@en ;
  rdfs:comment "Specifies a dimension used to evaluate common attributes"@en;
  rdfs:domain :Common ;
  rdfs:range owl:Thing .

:havingRole a owl:ObjectProperty ;
  rdfs:label "havingRole"@en ;
  rdfs:comment "Specifies a role"@en ;
  rdfs:domain :Everyone ;
  rdfs:range owl:Thing .

:havingRelationship a owl:ObjectProperty ;
  rdfs:label "havingRelationship"@en ;
  rdfs:comment "Specifies a type of relationship"@en ;
  rdfs:domain :Everyone ;
  rdfs:range owl:Thing .

:distance a owl:DatatypeProperty ;
  rdfs:label "distance"@en ;
  rdfs:comment "Specifies a relative 'degree of separation' from the context"@en ;
  rdfs:domain :Population ;
  rdfs:range xsd:nonNegativeInteger .

:confidence a owl:DatatypeProperty ;
  rdfs:label "confidence"@en ;
  rdfs:comment "Specifies a relative confidence level"@en ;
  rdfs:domain [
    a owl:Class;
      owl:unionOf ( :Common :Interested ) 
  ];
  rdfs:range [ 
    a rdfs:Datatype ;
    owl:onDatatype xsd:nonNegativeInteger ;
    owl:withRestrictions ( 
      [ xsd:maxInclusive "100"^^xsd:nonNegativeInteger ]
    )
  ] .