@prefix : <http://ns.jasnell.me/interval#> .
@prefix r: <http://ns.jasnell.me/interval#> .
@prefix owl: <http://www.w3.org/2002/07/owl#> .
@prefix rdf: <http://www.w3.org/1999/02/22-rdf-syntax-ns#> .
@prefix xml: <http://www.w3.org/XML/1998/namespace> .
@prefix xsd: <http://www.w3.org/2001/XMLSchema#> .
@prefix rdfs: <http://www.w3.org/2000/01/rdf-schema#> .
@base <http://ns.jasnell.me/interval#> .

<http://ns.jasnell.me/interval#> a owl:Ontology;
  rdfs:comment "A vocabulary for representing intervals"@en .

:lower a owl:DatatypeProperty, owl:FunctionalProperty ;
  rdfs:comment "The lower bound of an interval"@en;
  rdfs:domain :Interval .

:upper a owl:DatatypeProperty, owl:FunctionalProperty ;
  rdfs:comment "The upper bound of an interval"@en;
  rdfs:domain :Interval .

:step a owl:DatatypeProperty, owl:FunctionalProperty ;
  rdfs:comment "Specifies the significant step between values in the interval."@en;
  rdfs:domain :Interval .

:Interval a owl:Class ;
  rdfs:comment "Represents an interval of values with optional upper and lower bounds"@en .

:OpenInterval a owl:Class ;
  rdfs:comment "An interval open at both ends"@en ;
  rdfs:subClassOf :Interval .

:ClosedInterval a owl:Class ;
  rdfs:comment "An interval closed at both ends"@en ;
  rdfs:subClassOf :Interval .

:OpenClosedInterval a owl:Class ;
  rdfs:comment "An interval open at the lower bound, closed at the upper "@en ;
  rdfs:subClassOf :Interval .

:ClosedOpenInterval a owl:Class ;
  rdfs:comment "An interval open at the upper bound, closed at the lower "@en ;
  rdfs:subClassOf :Interval.

:LeftOpenInterval a owl:Class ;
  rdfs:comment "An interval open on the lower bound, with no upper bound"@en ;
  rdfs:subClassOf :Interval,
    [
      a owl:Restriction ;
        owl:onProperty :upper ;
        owl:cardinality "0"^^xsd:nonNegativeInteger .
    ] .

:LeftClosedInterval a owl:Class ;
  rdfs:comment "An interval closed on the lower bound, with no upper bound"@en ;
  rdfs:subClassOf :Interval,
    [
      a owl:Restriction ;
        owl:onProperty :upper ;
        owl:cardinality "0"^^xsd:nonNegativeInteger .
    ] .

:RightOpenInterval a owl:Class ;
  rdfs:comment "An interval open on the upper bound, with no lower bound"@en ;
  rdfs:subClassOf :Interval,
    [
      a owl:Restriction ;
        owl:onProperty :lower ;
        owl:cardinality "0"^^xsd:nonNegativeInteger .
    ] .

:RightClosedInterval a owl:Class ;
  rdfs:comment "An interval closed on the upper bound, with no lower bound"@en ;
  rdfs:subClassOf :Interval,
    [
      a owl:Restriction ;
        owl:onProperty :lower ;
        owl:cardinality "0"^^xsd:nonNegativeInteger .
    ] .

:EmptyInterval a :Interval ;
  rdfs:comment "The empty interval (contains no values)" .

:UnboundedInterval a :Interval ;
  rdfs:comment "An interval that is unbound at either end (contains all possible values)" .

## Example Instances

:PositiveIntegers a :LeftOpenInterval ;
  rdfs:comment "Represents all positive integers greater than zero" ;
  :lower "0"^^xsd:nonNegativeInteger ;
  :step "1"^^xsd:nonNegativeInteger .

:NonNegativeIntegers a :LeftClosedInterval ;
  rdfs:comment "Represents all non-negative integers greater than or equal to zero" ;
  :lower "0"^^xsd:nonNegativeInteger ;
  :step "1"^^xsd:nonNegativeInteger .

:NegativeIntegers a :RightClosedInterval ;
  rdfs:comment "Represents all negative integers" ;
  :upper "0"^^xsd:nonPositiveInteger ;
  :step "1"^^xsd:nonNegativeInteger .

:PositiveFloats a :LeftOpenInterval ;
  rdfs:comment "Represents all positive floating point numbers greater than zero" ;
  :lower "0"^^xsd:float.

:NonNegativeFloats a :LeftClosedInterval ;
  rdfs:comment "Represents all positive floating point numbers greater than or equal to zero" ;
  :lower "0"^^xsd:float .

:NegativeFloats a :RightClosedInterval ;
  rdfs:comment "Represents all negative floating point numbers" ;
  :upper "0"^^xsd:float .

:PositiveDoubles a :LeftOpenInterval ;
  rdfs:comment "Represents all positive double precision numbers greater than zero" ;
  :lower "0"^^xsd:double.

:NonNegativeDoubles a :LeftClosedInterval ;
  rdfs:comment "Represents all positive double precision numbers greater than or equal to zero" ;
  :lower "0"^^xsd:double .

:NegativeDoubles a :RightClosedInterval ;
  rdfs:comment "Represents all negative double precision numbers" ;
  :upper "0"^^xsd:double .

:PositiveDecimals a :LeftOpenInterval ;
  rdfs:comment "Represents all positive xsd:decimal numbers greater than zero" ;
  :lower "0"^^xsd:decimal.

:NonNegativeDecimals a :LeftClosedInterval ;
  rdfs:comment "Represents all positive xsd:decimal numbers greater than or equal to zero" ;
  :lower "0"^^xsd:decimal .

:NegativeDecimals a :RightClosedInterval ;
  rdfs:comment "Represents all negative xsd:decimal numbers" ;
  :upper "0"^^xsd:decimal .
